Trace.v
@@ -1,0 +1,167 @@
+Module Trace.
+
+CoInductive TraceOf (A : Type) : Type :=
+| finished : A -> TraceOf A
+| notfinished : A -> TraceOf A -> TraceOf A.
+
+Arguments finished {_} _.
+Arguments notfinished {_} _ _.
+
+Definition idTrace {A} (MM: TraceOf A) : TraceOf A :=
+  match MM with
+  | finished M => finished M
+  | notfinished M MM' => notfinished M  MM'
+  end.
+
+Lemma idTrace_eq : forall {A} (MM: TraceOf A), MM = idTrace MM.
+   destruct MM; reflexivity.
+Qed.
+
+Definition head {A} (MM : TraceOf A) : A :=
+  match MM with
+  | finished M => M
+  | notfinished M _ => M
+  end.
+
+Inductive InTrace {A} (m:A) : TraceOf A -> Prop :=
+| In_finished : InTrace m (finished m)
+| In_now : forall MM, InTrace m (notfinished m MM)
+| In_later : forall m' MM, InTrace m MM -> InTrace m (notfinished m' MM).
+
+Lemma head_InTrace :forall {A} (MM: TraceOf A), InTrace (head MM) MM.
+Proof.
+  intros.
+  destruct MM.
+  - constructor.
+  - simpl. constructor.
+Qed.
+
+CoFixpoint mapTrace {A B:Type} (f:A -> B) (T: TraceOf A) : TraceOf B :=
+  match T with
+  | finished a => finished (f a)
+  | notfinished a T' => notfinished (f a) (mapTrace f T')
+  end.
+
+CoInductive ForallTrace {A:Type} (P:A -> Prop) : TraceOf A -> Prop :=
+| Forall_finished : forall a, P a -> ForallTrace P (finished a)
+| Forall_notfinished : forall a T', P a -> ForallTrace P T' -> ForallTrace P (notfinished a T')
+.
+
+CoInductive TraceEq {A} : TraceOf A -> TraceOf A -> Prop :=
+| EqFin : forall m, TraceEq (finished m) (finished m)
+| EqCons : forall m mm1 mm2, TraceEq mm1 mm2 ->
+                             TraceEq (notfinished m mm1) (notfinished m mm2).
+
+CoFixpoint TraceApp {A} (T: TraceOf A) (TO: option (TraceOf A)) : TraceOf A :=
+  match T with
+  | finished a =>
+    match TO with
+    | Some a' => notfinished a a'
+    | None => T
+    end
+  | notfinished a T' => notfinished a (TraceApp T' TO)
+  end.
+
+Notation "T1 ^ T2" := (TraceApp T1 T2).
+
+Lemma TraceAppHead {A} :
+  forall (T1 T2 : TraceOf A) (TO : option (TraceOf A)),
+    T1 = T2 ^ TO -> head T1 = head T2.
+Proof.
+  intros T1 T2 TO App.
+  destruct T2 as [a | a T2'].
+  - rewrite App.
+    simpl.
+    destruct TO; simpl; auto.
+  - rewrite App.
+    simpl.
+    auto.
+Qed.
+
+(* TracePrefix MM1 MM2 says MM2 is a prefix of MM1. *)
+Definition TracePrefix {A} (T1 T2: TraceOf A): Prop :=
+  exists TO,
+    T1 = T2^TO.
+
+Notation "MM2 <<== MM1" := (TracePrefix MM1 MM2) (at level 80).
+
+(* Divide MM1 into MM2 ++ MMO such that MM2 is the longest prefix for which P holds on each element *)
+Definition TraceSpan {A} (P : A -> Prop) (MM1 MM2 : TraceOf A) (MMO : option (TraceOf A)) : Prop :=
+  MM1 = MM2^MMO /\ ForallTrace P MM2 /\
+  forall MM2', MM2' <<== MM1 ->
+    ForallTrace P MM2' ->
+    MM2' <<== MM2.
+
+(* MM2 is the longest prefix of MM1 for which P holds on each element. *)
+Definition LongestPrefix {A} (P : A -> Prop) (MM1 MM2 : TraceOf A) : Prop :=
+  exists MMO, TraceSpan P MM1 MM2 MMO.
+
+Inductive IsEnd {A} : TraceOf A -> A -> Prop :=
+| IsEndNow : forall a, IsEnd (finished a) a
+| IsEndLater : forall T a a', IsEnd T a -> IsEnd (notfinished a' T) a
+.
+
+(************************
+ Trace Lemmas and axioms 
+*************************)
+
+Lemma IsEndInTrace :
+  forall A (t:A) (T:TraceOf A),
+    IsEnd T t -> InTrace t T.
+Proof.
+  intros. induction H.
+  - constructor.
+  - constructor. auto.
+Qed.
+
+Lemma ForallInTrace :
+  forall A (f:A->Prop) T t,
+    InTrace t T ->
+    ForallTrace f T ->
+    f t.
+Proof.
+  intros. induction H; inversion H0; auto.
+Qed.
+
+Axiom TraceAppNone :
+  forall A (T : TraceOf A),
+    T = T^None.
+
+Lemma TracePrefix_refl :
+  forall A (T:TraceOf A),
+    T <<== T.
+Proof.
+  intros. exists None. apply TraceAppNone.
+Qed.
+
+Axiom TraceAppFinished :
+  forall A (a:A) (T:TraceOf A),
+    finished a ^ Some T = notfinished a T.
+
+Axiom IsEndAppFinish :
+  forall A (T:TraceOf A) (a:A),
+    IsEnd (T^Some (finished a)) a.
+
+Axiom ForallTraceApp :
+  forall A f (T1 T2 : TraceOf A),
+    ForallTrace f T1 ->
+    ForallTrace f T2 ->
+    ForallTrace f (T1^Some T2).
+
+Axiom TraceAppAssoc :
+  forall A (T1 T2 : TraceOf A) TO,
+    T1 ^ Some (T2 ^ TO) = (T1 ^ Some T2) ^ TO.
+
+Axiom ForallImplication :
+  forall A (P Q: A -> Prop) (T:TraceOf A),
+    (forall a, P a -> Q a) ->
+    ForallTrace P T ->
+    ForallTrace Q T.
+
+Axiom SpanRemainderNotProp :
+  forall A P (T T' T'': TraceOf A),
+    TraceSpan P T T' (Some T'') ->
+    ~ (P (head T'')).
+
+
+End Trace.
